geb-lean/GebLeanTests/Ramified.lean
@@ -8,6 +8,7 @@ import GebLeanTests.Ramified.HigherOrder
 import GebLeanTests.Ramified.OmegaShift
 import GebLeanTests.Ramified.Examples
 import GebLeanTests.Ramified.Algebras
+import GebLeanTests.Ramified.FirstOrder
 
 /-!
 # Ramified-recurrence test index
